Continue compiler.

Compiler.thy
@@ -1,5 +1,36 @@
 theory Compiler imports Big_Step Star begin
 
+(* Preliminaries *)
+
+declare [[coercion_enabled]]
+declare [[coercion "int :: nat \<Rightarrow> int"]]
+
+fun inth :: "'a list \<Rightarrow> int \<Rightarrow> 'a" (infixl "!!" 100) where
+  "(x # xs) !! i = (if i = 0 then x else xs !! (i - 1))"
+
+lemma inth_append [simp]:
+  "0 \<le> i \<Longrightarrow>
+  (xs @ ys) !! i = (if i < size xs then xs !! i else ys !! (i - size xs))"
+by (induction xs arbitrary: i) (auto simp: algebra_simps)
+
+(* Hide coercion int applied to length: *)
+abbreviation (output) "isize xs \<equiv> int (length xs)"
+notation isize ("size")
+
+(* The machine itself *)
+(* Realistically, we would map variable names to memory locations. *)
+
+datatype instr =
+  LOADI int
+| LOAD vname
+| ADD
+| STORE vname
+| JMP int
+| JMPLESS int (* Compare two topmost stack elements and jump if
+                 the second one is less. *)
+| JMPGE int   (* Compare two topmost stack elements and jump if
+                 the second one is greater or equal. *)
+
 
 
 end
